bump

ListCommon.v
@@ -1,7 +1,150 @@
-From mathcomp Require Import seq ssrbool eqtype choice.
-From SLF Require Import Sum Fun LabType Unary_IndexWithBounds.
+From mathcomp Require Import seq ssrbool eqtype choice ssreflect ssrfun zify.
+From SLF Require Import Sum Fun LabType.
 
 Import List.
+
+Fact nth_map_lt : forall [A B : Type] (da : A) (db : B) (f : A -> B) (l : list A) (n : nat)
+  (H : (n < length l)%nat),
+  nth n (map f l) db = f (nth n l da).
+Proof.
+  intros. revert l H. induction n as [ | n IH ]; intros.
+  { destruct l; simpl in H; try lia; auto. }
+  { destruct l; simpl in H; try lia; auto.
+    simpl. apply IH. lia. }
+Qed.
+
+Fact nth_In_int (l : list int) (n : int) :
+  (0 <= n < length l) -> In (nth (abs n) l 0) l.
+Proof. intros H. apply nth_In. math. Qed.
+
+(* TODO change the name of this section *)
+Section pure_facts.
+
+Context {A : Type}.
+
+Implicit Type l s : list A.
+(* Implicit Type i : A. *)
+
+Definition index (i : A) l : int. 
+Proof using.
+Admitted.
+Lemma index_nodup (def : A) i l : 
+  0 <= i < length l ->
+  List.NoDup l -> 
+    index (nth (abs i) l def) l = i.
+Proof.
+Admitted.
+
+Lemma in_take x l i : 0 <= i <= length l -> (In x (take (abs i) l)) = (index x l < i).
+Proof.
+Admitted.
+
+Lemma nth_index (def : A) x s : In x s -> nth (abs (index x s)) s def = x.
+Admitted.
+
+Lemma index_mem x s : (index x s < length s) = (In x s).
+Admitted.
+
+Lemma index_size x s : index x s <= length s.
+Proof. Admitted.
+
+Lemma indexG0 x s : 0 <= index x s.
+Proof. Admitted.
+
+Lemma memNindex x s :  ~In x s -> index x s = length s.
+Admitted.
+
+Definition list_interval (lb rb : nat) l :=
+  take (rb - lb)%nat (drop lb l).
+
+Lemma list_interval_length (lb rb : int) l :
+  0 <= lb <= rb -> rb <= length l -> length (list_interval (abs lb) (abs rb) l) = rb - lb :> int.
+Admitted.
+
+Lemma list_interval_nth (def : A) (x lb rb : int) l :
+  0 <= lb <= rb -> rb <= length l -> 0 <= x < rb - lb ->
+  nth (abs (lb + x)) l def = nth (abs x) (list_interval (abs lb) (abs rb) l) def.
+Admitted.
+
+End pure_facts.
+
+Section list_of_fun.
+
+(* some customized theory of from functions to lists *)
+Lemma list_of_fun [A : Type] (f : int -> A) (n : int) (H : 0 <= n) :
+  @sigT (list A) (fun l =>
+    (length l = n :> int /\ (forall (i : int) (def : A), 0 <= i < n -> nth (abs i) l def = f i))).
+Proof.
+  remember (abs n) as nn eqn:E.
+  revert n H E. induction nn as [ | nn IH ]; intros.
+  { assert (n = 0) as -> by math. exists (@nil A). split; auto. intros; math. }
+  { assert (nn = abs (n - 1)) as Hq by math. apply IH in Hq; try math.
+    destruct Hq as (la & H1 & H2). exists (app la (f (n - 1) :: nil)).
+    rewrite -> app_length. split; simpl; try math.
+    intros i def Hin. destruct (Z.leb (n - 1) i) eqn:E2.
+    { apply Z.leb_le in E2. replace i with (n-1) in * by math. 
+      replace (abs (n-1)) with (length la) by math. now rewrite nth_middle. }
+    { apply Z.leb_gt in E2. rewrite app_nth1. 1: apply H2. all: math. } }
+Qed.
+
+Definition list_of_fun' [A : Type] (f : int -> A) (n : int) :
+  @sigT (list A) (fun l =>
+    (length l = abs n :> int /\ (forall (i : int) (def : A), 0 <= i < abs n -> nth (abs i) l def = f i))).
+apply list_of_fun. math. Defined.
+
+Fact lof_make_constfun [A : Type] (c : A) (n : int) :
+  (projT1 (list_of_fun' (fun _ => c) n)) = repeat c (abs n).
+Proof.
+  destruct (list_of_fun' _ _) as (l & Hlen & HH). simpl.
+  apply nth_ext with (d:=c) (d':=c).
+  1: rewrite repeat_length; math.
+  intros i Hi. 
+  rewrite -> nth_repeat; try math. rewrite <- HH with (i:=i) (def:=c) at 2; try math.
+  f_equal; math.
+Qed.
+
+(* TODO possibly change this name? *)
+Definition lof f N := projT1 (@list_of_fun' int f N).
+
+Lemma nth_lof f N i : 
+  0 <= i < abs N -> nth (abs i) (lof f N) 0 = f i.
+Proof. unfold lof. destruct (list_of_fun' _ _) as (l1 & Hlen1 & Hl1); simpl. auto. Qed.
+
+Lemma nth_lof' f N i :
+  0 <= N -> 0 <= i < N -> nth (abs i) (lof f N) 0 = f i.
+Proof. intros ??. apply nth_lof. math. Qed.
+
+Lemma length_lof f N : 
+  0 <= N -> length (lof f N) = N :> int.
+Proof. unfold lof. destruct (list_of_fun' _ _) as (l1 & Hlen1 & Hl1); simpl. math. Qed.
+
+Lemma length_lof' f N : 
+  length (lof f N) = abs N :> nat.
+Proof. unfold lof. destruct (list_of_fun' _ _) as (l1 & Hlen1 & Hl1); simpl. math. Qed.
+
+Lemma In_lof_id N a : In a (lof id N) -> 0 <= a < abs N.
+Proof.
+  unfold lof. destruct (list_of_fun' _ _) as (l1 & Hlen1 & Hl1); simpl.
+  intros H. apply In_nth with (d:=0) in H. destruct H as (n & Hlt & <-).
+  replace n with (abs n) by math. rewrite Hl1; math.
+Qed.
+
+Lemma lof_indices {A : Type} (a : A) (f : int -> A) (g : int -> int) n :
+  projT1 (list_of_fun' (f \o g) n) = map f (lof g n).
+Proof.
+  destruct (list_of_fun' _ _) as (l1 & Hlen1 & Hl1); simpl.
+  pose proof (length_lof' g n) as Hlen2.
+  apply (nth_ext _ _ a a). 
+  1: rewrite map_length; math.
+  intros n0 Hlt. replace n0 with (abs n0) by math.
+  rewrite Hl1 ?(nth_map_lt 0) ?nth_lof //; try math.
+Qed.
+
+Corollary lof_indices' {A : Type} (a : A) (f : int -> A) n :
+  projT1 (list_of_fun' f n) = map f (lof id n).
+Proof. by rewrite <- lof_indices. Qed.
+
+End list_of_fun.
 
 Definition sorted (l : list int) : Prop. Admitted.
 Definition max (l : list int) : int. Admitted.
